@prefix pmdcat: <http://publishmydata.com/pmdcat#> .
@prefix dc: <http://purl.org/dc/elements/1.1/> .
@prefix dcat: <http://www.w3.org/ns/dcat#> .
@prefix dct: <http://purl.org/dc/terms/> .
@prefix dctype: <http://purl.org/dc/dcmitype/> .
@prefix foaf: <http://xmlns.com/foaf/0.1/> .
@prefix owl: <http://www.w3.org/2002/07/owl#> .
@prefix rdf: <http://www.w3.org/1999/02/22-rdf-syntax-ns#> .
@prefix rdfs: <http://www.w3.org/2000/01/rdf-schema#> .
@prefix schema: <http://schema.org/> .
@prefix skos: <http://www.w3.org/2004/02/skos/core#> .
@prefix xsd: <http://www.w3.org/2001/XMLSchema#> .
@prefix qb: <http://purl.org/linked-data/cube#> .
@prefix void: <http://rdfs.org/ns/void#> .
@prefix markdown: <https://www.w3.org/ns/iana/media-types/text/markdown#> .

<http://publishmydata.com/pmdcat>
  rdf:type owl:Ontology ;
  rdfs:label "Publish My Data Catalog vocabulary" ;
  rdfs:comment "PMDCat builds on https://w3c.github.io/dxwg/dcat/ to refine some terms in dcat2 for use in publishmydata." ;
 .

pmdcat:Catalog
  rdfs:subClassOf dcat:Catalog ;
  rdfs:label "A PublishMyData Catalog" ;
  .

pmdcat:DatasetContents
    a rdf:Class ;
    rdfs:label "Dataset Contents" ;
    rdfs:comment "The contents of a Dataset." ;
  .

pmdcat:Dataset
  rdfs:subClassOf dcat:Dataset ;
  rdfs:label "Dataset" ;
  rdfs:comment "The base type of all PublishMyData datasets"  ;
  .


#pmdcat:FileDataset
#  rdfs:subClassOf dcat:Dataset ;
#  rdfs:label "File Dataset" ;
#  rdfs:comment "A PublishMyData dataset which stores a file attachment" ;
#  .

#pmdcat:URLDataset
#  rdfs:subClassOf dcat:Dataset ;
#  rdfs:label "URL Dataset" ;
#  rdfs:comment "A PublishMyData dataset which points to a remote URL" ;
#  .

#pmdcat:LinkedDataset
#    rdfs:subClassOf pmdcat:DatasetContents ;
#    rdfs:label "Linked Data Dataset" ;
#    rdfs:comment "A PublishMyData dataset which stores Linked Data, and has a root node which we can point to (e.g. a cube)." ;
#    .

pmdcat:DataCube
    rdfs:subClassOf pmdcat:DatasetContents ;
#    rdfs:subClassOf pmdcat:LinkedDataset ;
    rdfs:label "DataCube" ;
    rdfs:comment "A PublishMyData compatible Linked Data Cube"
    .

pmdcat:GraphDatasetContents
    rdfs:subClassOf pmdcat:DatasetContents ;
    rdfs:label "Dataset" ;
    rdfs:comment "Contents of a PublishMyData dataset which is just a graph of RDF, with no obvious root node." ;
    .

#pmdcat:Vocabulary
#    rdfs:subClassOf pmdcat:DatasetContents ;
#    rdfs:label "Vocabulary" ;
#    rdfs:comment "Contents of a PublishMyData dataset which is an RDF Vocabulary." ;
#  .

pmdcat:Ontology
#   rdfs:subClassOf pmdcat:Vocabulary ;
    rdfs:subClassOf pmdcat:DatasetContents ;
    rdfs:label "Ontology" ;
    rdfs:comment "Contents of a PublishMyData dataset which is an RDF Ontology." ;
    .

pmdcat:ConceptScheme
#   rdfs:subClassOf pmdcat:Vocabulary ;
    rdfs:subClassOf pmdcat:DatasetContents ;
    rdfs:label "Concept Scheme" ;
    rdfs:comment "Contents of a PublishMyData dataset which is an RDF Concept Scheme." ;
    .

#pmdcat:DatasetCSVDownloadService
#  rdfs:subClassOf dcat:DataService ;
#  rdfs:label "PublishMyData Dataset CSV Download Service" ;
#  rdfs:comment "A PublishMyData Data service for downloading CSV files from RDFBaseDatasets" ;
#  .

#pmdcat:DatasetRDFDownloadService
#  rdfs:subClassOf dcat:DataService ;
#  rdfs:label "PublishMyData Dataset RDF Download Service" ;
#  rdfs:comment "A PublishMyData Data service for downloading RDF files from RDFBaseDatasets" ;
#  .

#pmdcat:dependsOn
#  rdfs:subPropertyOf void:Vocabulary ;
#  rdfs:label "dependsOn" ;
#  rdfs:comment "On what other pmdcat datasets does this one depend?" ;
#  rdfs:range pmdcat:Dataset ;
#  rdfs:domain pmdcat:Dataset ;
#  .

pmdcat:graph
  a rdf:Property ;
  rdfs:label "graph" ;
  rdfs:comment "What named graph(s) are used to store this dataset" ;
  rdfs:domain pmdcat:Dataset .
  #rdfs:range pmdcat:DatasetContents .


pmdcat:datasetContents
  a rdf:Property ;
    rdfs:label "datasetContents" ;
  rdfs:comment "An RDF Datasets contents, either points to a graph containing the datasets triples, or the RDF datasets root resource node, e.g. in the case of native RDF dataset types such as qb:Dataset.  This allows catalogue metadata to be separated from the datasets contents." ;
  rdfs:domain pmdcat:Dataset ;
  rdfs:range pmdcat:DatasetContents .

pmdcat:metadataGraph
  a rdf:Property ;
  rdfs:label "metadataGraph" ;
  rdfs:comment "What named graph(s) are used to store the metadata of a dataset" ;
  rdfs:domain dcat:CatalogRecord ;
  .

pmdcat:markdownDescription
  rdfs:label "Markdown Description" ;
  rdfs:comment "A version of the dataset description with markdown formatting" ;
  rdfs:subPropertyOf dct:description ;
  rdfs:domain pmdcat:Dataset ;
  rdfs:range markdown:Resource ;
  .
